pulse/lib/pulse/lib/Pulse.Lib.SpinLock.fst
@@ -15,91 +15,207 @@
 *)
 
 module Pulse.Lib.SpinLock
+
 open Pulse.Lib.Pervasives
+open Pulse.Lib.CancellableInvariant
+
+
 module Box = Pulse.Lib.Box
 module U32 = FStar.UInt32
+module GR = Pulse.Lib.GhostReference
 
-// let maybe (b:bool) (p:vprop) =
-//     if b then p else emp
+let big_star (p q : vprop)
+: Lemma
+    (requires is_big p /\ is_big q)
+    (ensures is_big (p ** q))
+    [SMTPat (is_big (p ** q))] = big_star p q
 
-// let lock_inv (r:ref U32.t) (p:vprop) =
-//   exists* v. pts_to r v ** maybe (v = 0ul) p
+let big_exists (#a:Type u#a) (p: a -> vprop)
+: Lemma
+    (requires forall x. is_big (p x))
+    (ensures is_big (op_exists_Star p))
+    [SMTPat (is_big (op_exists_Star p))] = big_exists p
 
-let lock = admit ()
+let lock_inv_aux (r:ref U32.t) (gr:GR.ref U32.t) (v:vprop) : (w:vprop { is_big v ==> is_big w })  =
+  exists* i p. pts_to r #full_perm i **
+               GR.pts_to gr #p i **
+               (if i = 0ul then v else emp) **
+               pure ((i == 0ul ==> p == full_perm) /\
+                     (i =!= 0ul ==> p == half_perm full_perm)) 
 
-// noeq
-// type lock (p:vprop) = {
-//   r:ref U32.t;
-//   i:inv (lock_inv r p);
-// }
+let lock_inv (r:ref U32.t) (gr:GR.ref U32.t) (v:vprop) : vprop =
+  lock_inv_aux r gr v
 
-// ```pulse
-// fn new_lock' (p:vprop)
-// requires p
-// returns l:lock p
-// ensures emp
-// {
-//    let r = Box.alloc 0ul;
-//    Box.to_ref_pts_to r;
-//    fold (maybe (0ul = 0ul) p);
-//    fold (lock_inv (Box.box_to_ref r) p);
-//    let i = new_invariant (lock_inv (Box.box_to_ref r) p);
-//    let l = { r = Box.box_to_ref r; i };
-//    l
-// }
-// ```
-let new_lock = admit ()  //new_lock'
+let is_big_lock_inv (r:ref U32.t) (gr:GR.ref U32.t) (v:vprop)
+  : Lemma (is_big v ==> is_big (lock_inv r gr v)) = ()
 
-// ```pulse
-// fn rec acquire' #p (l:lock p)
-// requires emp
-// ensures p
-// {
-//   let b = 
-//     with_invariants l.i
-//     returns b:bool
-//     ensures maybe b p 
-//     {
-//       unfold lock_inv;
-//       let b = cas l.r 0ul 1ul;
-//       if b
-//       { 
-//         elim_cond_true _ _ _;
-//         with _b. rewrite (maybe _b p) as p;
-//         fold (maybe false p);
-//         rewrite (maybe false p) as (maybe (1ul = 0ul) p);
-//         fold (lock_inv l.r p);
-//         fold (maybe true p);
-//         true
-//       }
-//       else
-//       {
-//         elim_cond_false _ _ _;
-//         fold (lock_inv l.r p);
-//         fold (maybe false p);
-//         false
-//       }
-//     };
-//   if b { rewrite (maybe b p) as p; }
-//   else { rewrite (maybe b p) as emp; acquire' l }
-// }
-// ```
-let acquire = admit ()
+noeq
+type lock = {
+  r : ref U32.t;
+  gr : GR.ref U32.t;
+  i : cinv;
+}
 
+let lock_alive l #p v =
+  inv l.i.i (cancellable l.i.t (lock_inv l.r l.gr v)) ** active p l.i.t
 
-// ```pulse
-// fn release' #p (l:lock p)
-// requires p
-// ensures emp
-// {
-//   with_invariants l.i {
-//     unfold lock_inv;
-//     write_atomic l.r 0ul;
-//     drop_ (maybe _ _); //double release
-//     fold (maybe (0ul = 0ul) p);
-//     fold (lock_inv l.r p);
-//   }
-// }
-// ```
-let release = admit ()
+let lock_acquired l #p v =
+  inv l.i.i (cancellable l.i.t (lock_inv l.r l.gr v)) ** active p l.i.t ** GR.pts_to l.gr #(half_perm full_perm) 1ul
 
+```pulse
+fn new_lock_aux (v:vprop { is_big v })
+  requires v
+  returns l:lock
+  ensures lock_alive l v
+{
+  let r = alloc 0ul;
+  let gr = GR.alloc 0ul;
+  rewrite v as (if 0ul = 0ul then v else emp);
+  fold (lock_inv_aux r gr v);
+  fold (lock_inv r gr v);
+  is_big_lock_inv r gr v;
+  let i = new_cancellable_invariant (lock_inv r gr v);
+  let l = { r; gr; i };
+  rewrite each r as l.r;
+  rewrite each gr as l.gr;
+  rewrite each i as l.i;
+  fold (lock_alive l #full_perm v);
+  l
+}
+```
+
+let new_lock = new_lock_aux
+
+```pulse
+fn rec acquire_aux (#v:vprop) (#p:perm) (l:lock)
+  requires lock_alive l #p v
+  ensures v **  lock_acquired l #p v
+{
+  unfold (lock_alive l #p v);
+  let b =
+    with_invariants l.i.i
+      returns b:bool
+      ensures active p l.i.t **
+              (if b then v ** GR.pts_to l.gr #(half_perm full_perm) 1ul else emp) {
+      take l.i.t;
+      unfold lock_inv;
+      unfold lock_inv_aux;
+      let b = cas l.r 0ul 1ul;
+      if b {
+        elim_cond_true _ _ _;
+        GR.(l.gr := 1ul);
+        GR.share2 l.gr;
+        rewrite emp as (if (1ul = 0ul) then v else emp);
+        fold (lock_inv_aux l.r l.gr v);
+        fold (lock_inv l.r l.gr v);
+        give l.i.t;
+        assert (cancellable l.i.t (lock_inv l.r l.gr v) **
+                active p l.i.t **
+                GR.pts_to l.gr #(half_perm full_perm) 1ul **
+                v);
+        let b = true;
+        rewrite (v ** GR.pts_to l.gr #(half_perm full_perm) 1ul)
+             as (if b then v ** GR.pts_to l.gr #(half_perm full_perm) 1ul else emp);
+        b
+      } else {
+        elim_cond_false _ _ _;
+        fold (lock_inv_aux l.r l.gr v);
+        fold (lock_inv l.r l.gr v);
+        give l.i.t;
+        assert (cancellable l.i.t (lock_inv l.r l.gr v) **
+                active p l.i.t);
+        let b = false;
+        rewrite emp as
+                (if b then v ** GR.pts_to l.gr #(half_perm full_perm) 1ul else emp);
+        b
+      }
+    };
+
+  if b {
+    rewrite (if b then v ** GR.pts_to l.gr #(half_perm full_perm) 1ul else emp) as
+            (v ** GR.pts_to l.gr #(half_perm full_perm) 1ul);
+    fold (lock_acquired l #p v);
+  } else {
+    rewrite (if b then v ** GR.pts_to l.gr #(half_perm full_perm) 1ul else emp) as
+            emp;
+    fold (lock_alive l #p v);
+    acquire_aux l
+  }
+}
+```
+
+let acquire = acquire_aux
+
+```pulse
+fn release_aux (#v:vprop) (#p:perm) (l:lock)
+  requires v ** lock_acquired l #p v
+  ensures lock_alive l #p v
+{
+  unfold (lock_acquired l #p v);
+
+  with_invariants l.i.i
+    returns _:unit
+    ensures active p l.i.t {
+    take l.i.t;
+    unfold (lock_inv l.r l.gr v);
+    unfold (lock_inv_aux l.r l.gr v);
+    GR.pts_to_injective_eq l.gr;
+    GR.gather2 l.gr;
+    rewrite (if (1ul = 0ul) then v else emp) as emp;
+    write_atomic l.r 0ul;
+    GR.(l.gr := 0ul);
+    fold (lock_inv_aux l.r l.gr v);
+    fold (lock_inv l.r l.gr v);
+    give l.i.t;
+  };
+
+  fold (lock_alive l #p v)
+}
+```
+
+let release = release_aux
+
+```pulse
+ghost
+fn share_aux (#v:vprop) (#p:perm) (l:lock)
+  requires lock_alive l #p v
+  ensures lock_alive l #(half_perm p) v ** lock_alive l #(half_perm p) v
+  opens emp_inames
+{
+  unfold (lock_alive l #p v);
+  share l.i.t;
+  dup_inv l.i.i (cancellable l.i.t (lock_inv l.r l.gr v));  // make this arg implicit
+  fold (lock_alive l #(half_perm p) v);
+  fold (lock_alive l #(half_perm p) v)
+} 
+```
+
+let share = share_aux
+
+```pulse
+ghost
+fn gather_aux (#v:vprop) (#p:perm) (l:lock)
+  requires lock_alive l #(half_perm p) v ** lock_alive l #(half_perm p) v
+  ensures lock_alive l #p v
+  opens emp_inames
+{
+  unfold (lock_alive l #(half_perm p) v);
+  unfold (lock_alive l #(half_perm p) v);
+  gather l.i.t;
+  fold (lock_alive l #p v);
+  drop_ (inv _ _)
+} 
+```
+
+let gather = gather_aux
+
+```pulse
+fn free_aux (#v:vprop) (l:lock)
+  requires lock_alive l #full_perm v
+  ensures v
+{
+  admit ()
+}
+```
+
+let free = free_aux
